examples/Hoare/Imp.v
@@ -1,0 +1,401 @@
+Require Import Coq.Strings.String.
+Require Import ExtLib.Structures.Applicative.
+Require Import ExtLib.Data.Fun.
+Require Import McExamples.Hoare.ILogic.
+
+Set Implicit Arguments.
+Set Strict Implicit.
+
+Local Instance Applicative_Fun A : Applicative (Fun A) :=
+{ pure := fun _ x _ => x
+; ap := fun _ _ f x y => (f y) (x y)
+}.
+
+Module Type ImpLang.
+
+  Definition var := string.
+  Definition value := nat.
+
+  (* States *)
+  Parameter locals : Type.
+  Parameter locals_upd : var -> value -> locals -> locals.
+  Parameter locals_get : var -> locals -> value.
+
+  (* Expressions *)
+  Parameter iexpr : Type.
+  Parameter iConst : value -> iexpr.
+  Parameter iVar : var -> iexpr.
+  Parameter iPlus : iexpr -> iexpr -> iexpr.
+  Parameter iEq : iexpr -> iexpr -> iexpr.
+  Parameter iLt : iexpr -> iexpr -> iexpr.
+
+  Parameter eval_iexpr : iexpr -> locals -> value.
+
+  (* Commands *)
+  Parameter icmd : Type.
+
+  Parameter Skip : icmd.
+  Parameter Seq : icmd -> icmd -> icmd.
+  Parameter Assign : var -> iexpr -> icmd.
+  Parameter If : iexpr -> icmd -> icmd -> icmd.
+
+  (* Logic for the Axiomatic Semantics *)
+  Universe Uall Ulogic.
+  Parameter HProp : Type@{Ulogic}. (* Predicates over the global state *)
+
+  Parameter ILogicOps_HProp : ILogicOps@{Uall Ulogic} HProp.
+  Parameter ILogic_HProp : ILogic HProp.
+  Parameter EmbedOp_Prop_HProp : EmbedOp Prop HProp.
+  Parameter Embed_Prop_HProp : Embed Prop HProp.
+
+  Parameter SProp : Type@{Ulogic}. (* The specification logic *)
+
+  Parameter ILogicOps_SProp : ILogicOps@{Uall Ulogic} SProp.
+  Parameter ILogic_SProp : ILogic SProp.
+  Parameter EmbedOp_Prop_SProp : EmbedOp Prop SProp.
+  Parameter Embed_Prop_SProp : Embed Prop SProp.
+
+  Definition lprop := locals -> HProp.
+
+  Instance ILogicOps_lprop : ILogicOps@{Uall Ulogic} lprop := _.
+  Instance ILogic_lprop : ILogic lprop := _.
+
+  Instance EmbedOp_HProp_lprop : EmbedOp@{Ulogic Ulogic} HProp lprop := _.
+  Instance Embed_HProp_lprop : Embed HProp lprop := _.
+
+  (* Axiomatics Semantics *)
+  Parameter triple : lprop -> icmd -> lprop -> SProp.
+
+  (** Consequence **)
+  Axiom Conseq_rule
+  : forall G P P' Q' Q c,
+      G |-- embed (P |-- P') ->
+      G |-- embed (Q' |-- Q) ->
+      G |-- triple P' c Q' ->
+      G |-- triple P c Q.
+
+  (** Quantifier Rules **)
+  Axiom triple_exL
+  : forall G P c Q,
+      (G |-- Forall x : value, triple (P x) c Q) ->
+      G |-- triple (lexists P) c Q.
+
+  Axiom triple_pureL
+  : forall (P : Prop) G c Q R,
+      (G //\\ embed P |-- triple Q c R) ->
+      G |-- triple (land (embed (embed P)) Q) c R.
+
+  Lemma entails_exL
+    : forall (P : value -> locals -> HProp) Q,
+      (forall x, P x |-- Q) ->
+      lexists P |-- Q.
+  Proof.
+    intros. apply lexistsL. eassumption.
+  Qed.
+
+  Lemma go_lower
+    : forall (P Q : lprop) (G : SProp),
+      G |-- lforall (fun x : locals => embed (P x |-- Q x)) ->
+      G |-- @embed Prop SProp EmbedOp_Prop_SProp (P |-- Q).
+  Proof.
+    intros.
+    etransitivity; [ eassumption | clear ].
+    unfold embed. simpl.
+    etransitivity; [ eapply embedlforall | ].
+    simpl. reflexivity.
+  Qed.
+  Lemma go_lower_raw
+    : forall (P Q : lprop),
+      (forall x : locals, P x |-- Q x) ->
+      (P |-- Q).
+  Proof.
+    red; simpl; intros.
+    eapply H.
+  Qed.
+
+  (** Skip **)
+  Axiom Skip_rule_refl
+  : forall G P,
+      G |-- triple P Skip P.
+
+  Theorem Skip_rule
+  : forall G P Q,
+      G |-- embed (P |-- Q) ->
+      G |-- triple P Skip Q.
+  Proof.
+    intros.
+    eapply Conseq_rule; [ | | eapply Skip_rule_refl ].
+    - eassumption.
+    - eapply embed_drop.
+      admit.
+  Admitted.
+
+  (** Sequence **)
+  Axiom Seq_rule
+  : forall G P Q R c1 c2,
+      G |-- triple P c1 Q ->
+      G |-- triple Q c2 R ->
+      G |-- triple P (Seq c1 c2) R.
+
+  Axiom SeqA_rule
+  : forall G P Q c1 c2 c3,
+      G |-- triple P (Seq c1 (Seq c2 c3)) Q ->
+      G |-- triple P (Seq (Seq c1 c2) c3) Q.
+
+  (** Assignment **)
+  Axiom Assign_rule
+  : forall G P x e,
+    G |-- triple P
+                 (Assign x e)
+                 (fun l => Exists v' : value,
+                             P  (locals_upd x v' l) //\\
+                             embed (locals_get x l = eval_iexpr e (locals_upd x v' l))).
+
+  (** Assert **)
+  Parameter Assert : lprop -> icmd.
+
+  Axiom Assert_rule
+  : forall G (Q : lprop),
+      G |-- triple Q (Assert Q) Q.
+
+  (** If **)
+  Axiom If_rule
+  : forall (G : SProp) (P Q : lprop) (x : iexpr) (c1 c2 : icmd),
+      G |-- triple (P //\\ (fun l : locals => embed (eval_iexpr x l <> 0))) c1 Q ->
+      G |-- triple (P //\\ (fun l : locals => embed (eval_iexpr x l = 0))) c2  Q ->
+      G |-- triple P (If x c1 c2) Q.
+
+
+  Definition update {T} (f : locals -> locals) (m : locals -> T) (l : locals)
+  : T := m (f l).
+
+End ImpLang.
+
+(*
+Definition local_Prop_lprop (P : Fun locals Prop) : lprop :=
+  fun l => embed (P l).
+
+Definition exprProp (P : value -> Prop) (e : locals -> value) : lprop :=
+  local_Prop_lprop (fun l => P (e l)).
+
+(*
+Eval cbv beta iota zeta delta [ exprProp local_Prop_lprop ] in
+  forall G (P Q : lprop) x c1 c2,
+    G |-- triple (P //\\ exprProp (fun v => v <> 0) (eval_iexpr x)) c1 Q ->
+    G |-- triple (P //\\ exprProp (fun v => v = 0) (eval_iexpr x)) c2 Q ->
+    G |-- triple P (If x c1 c2) Q.
+*)
+
+
+
+(** Read **)
+Parameter Read : var -> iexpr -> icmd.
+
+Parameter PtsTo : value -> value -> HProp.
+
+Axiom Read_rule
+: forall G (P : lprop) x e (v : locals -> value),
+    (G |-- embed (P |-- ap (T := Fun locals) (ap (pure PtsTo) (eval_iexpr e)) v ** ltrue)) ->
+    G |-- triple P
+                 (Read x e)
+                 (fun l =>
+                    Exists v' : value,
+                          P (locals_upd x v' l)
+                    //\\  embed (locals_get x l = v (locals_upd x v' l))).
+
+(** Write **)
+Parameter Write : iexpr -> iexpr -> icmd.
+
+Axiom Write_rule
+: forall G (P Q : lprop) p v,
+    G |-- embed (P |-- Exists v', ap (T := Fun locals) (ap (pure PtsTo) (eval_iexpr p)) (pure v') ** Q) ->
+    G |-- triple P
+           (Write p v)
+           (ap (T := Fun locals) (ap (pure PtsTo) (eval_iexpr p)) (eval_iexpr v) ** Q).
+
+(** Continuation Rules **)
+(** Seq_rule **)
+Theorem Assign_seq_rule
+: forall G P Q x e c,
+    G |-- triple (Exists v' : value, (fun l =>
+                             P  (locals_upd x v' l) //\\
+                             embed (locals_get x l = eval_iexpr e (locals_upd x v' l)))) c Q ->
+    G |-- triple P
+                 (Seq (Assign x e) c)
+                 Q.
+Proof.
+  intros. eapply Seq_rule. eapply Assign_rule. eassumption.
+Qed.
+
+Theorem Assign_tail_rule
+: forall G P Q x e,
+    G |-- embed (Exists v' : value, (fun l => 
+                             P  (locals_upd x v' l) //\\
+                             embed (locals_get x l = eval_iexpr e (locals_upd x v' l))) |-- Q) ->
+    G |-- triple P (Assign x e) Q.
+Proof.
+  intros.
+  eapply Conseq_rule. 3: eapply Assign_rule.
+  2: eapply H.
+  admit.
+Qed.
+
+Theorem Read_seq_rule
+: forall G (P Q : lprop) x e (v : locals -> value) c,
+    (G |-- embed (P |-- ap (T := Fun locals) (ap (pure PtsTo) (eval_iexpr e)) v ** ltrue)) ->
+    (G |-- triple (Exists v' : value, fun l =>
+                          P (locals_upd x v' l)
+                    //\\  embed (locals_get x l = v (locals_upd x v' l))) c Q) ->
+    G |-- triple P (Seq (Read x e) c) Q.
+Proof.
+  intros. eapply Seq_rule. eapply Read_rule. eapply H. assumption.
+Qed.
+
+Theorem Read_tail_rule
+: forall G (P Q : lprop) x e (v : locals -> value),
+    (G |-- embed (P |-- ap (T := Fun locals) (ap (pure PtsTo) (eval_iexpr e)) v ** ltrue)) ->
+    (G |-- embed (Exists v' : value, (fun l =>
+                          P (locals_upd x v' l)
+                    //\\  embed (locals_get x l = v (locals_upd x v' l))) |-- Q)) ->
+    G |-- triple P (Read x e) Q.
+Proof.
+  intros. eapply Conseq_rule; [ | | eapply Read_rule ].
+  3: eassumption. admit. eassumption.
+Qed.
+
+Theorem Write_seq_rule
+: forall G (P Q R : lprop) p v c,
+    (G |-- embed (P |-- Exists v', ap (T := Fun locals) (ap (pure PtsTo) (eval_iexpr p)) (pure v') ** Q)) ->
+    (G |-- triple (ap (T := Fun locals) (ap (pure PtsTo) (eval_iexpr p)) (eval_iexpr v) ** Q) c R) ->
+    G |-- triple P (Seq (Write p v) c) R.
+Proof.
+  intros. eapply Seq_rule. eapply Write_rule. eassumption. eassumption.
+Qed.
+
+Theorem Write_tail_rule
+: forall G (P Q R : lprop) p v,
+    G |-- embed (P |-- Exists v', ap (T := Fun locals) (ap (pure PtsTo) (eval_iexpr p)) (pure v') ** Q) ->
+    (G |-- embed ((ap (T := Fun locals) (ap (pure PtsTo) (eval_iexpr p)) (eval_iexpr v) ** Q) |-- R)) ->
+    G |-- triple P (Write p v) R.
+Proof.
+  intros. eapply Conseq_rule. 3: eapply Write_rule. 2: eassumption. 2: eassumption. admit.
+Qed.
+
+Theorem Skip_seq_rule
+: forall G P Q c,
+    G |-- triple P c Q ->
+    G |-- triple P (Seq Skip c) Q.
+Proof.
+  intros. eapply Seq_rule. eapply Skip_rule_refl. eassumption.
+Qed.
+
+Definition Skip_tail_rule := Skip_rule.
+
+Theorem Assert_seq_rule
+: forall G P Q A c,
+    G |-- embed (P |-- A) ->
+    G |-- triple A c Q ->
+    G |-- triple P (Seq (Assert A) c) Q.
+Proof.
+  intros. eapply Seq_rule. eapply Assert_rule. eassumption. eassumption.
+Qed.
+
+Theorem Assert_tail_rule
+: forall G P Q A,
+    G |-- embed (P |-- A) ->
+    G |-- embed (A |-- Q) ->
+    G |-- triple P (Assert A) Q.
+Proof.
+  intros. eapply Conseq_rule; try eassumption.
+  eapply Assert_rule. admit.
+Qed.
+
+
+
+
+
+(** While **)
+Parameter While : iexpr -> icmd -> icmd.
+
+Axiom While_rule
+: forall G (P Q I : lprop) t c,
+    G |-- embed (P |-- I) ->
+    G |-- triple (I //\\ exprProp (fun v => v <> 0) (eval_iexpr t)) c I ->
+    G |-- embed (I //\\ exprProp (fun v => v = 0) (eval_iexpr t) |-- Q) ->
+    G |-- triple P (While t c) Q.
+
+
+Parameter WhileI : lprop -> iexpr -> icmd -> icmd.
+
+Axiom WhileI_rule
+: forall G (P Q I : lprop) t c,
+    G |-- embed (P |-- I) ->
+    G |-- triple (I //\\ exprProp (fun v => v <> 0) (eval_iexpr t)) c I ->
+    G |-- embed (I //\\ exprProp (fun v => v = 0) (eval_iexpr t) |-- Q) ->
+    G |-- triple P (WhileI I t c) Q.
+
+(*
+(** Theorem, some manipulation **)
+Axiom liftEx
+: forall (t : Type) G P (Q : lprop),
+    G |-- @lexists _ _ t (fun v => embed (P v |-- Q)) ->
+    G |-- embed (@lexists _ _ t P |-- Q).
+*)
+
+
+
+(**
+(** Function Calls **)
+
+Definition function_name := string.
+
+Parameter Call : function_name -> iexpr -> icmd.
+
+Axiom function_spec : function_name -> (nat -> lprop) -> (nat -> lprop) -> SProp.
+
+Axiom Call_rule
+: forall G (P Q : lprop) (P' Q' : nat -> lprop) F f e v,
+    G |-- embed (P |-- ap (T := Fun locals) (ap (pure PtsTo) (eval_iexpr e)) v ** ltrue) ->
+    G |-- function_spec f P' Q' -> (** Get the method spec **)
+    G |-- embed (P |-- ap (T := Fun locals) (fun l v => P' v l) v ** F) -> (* P |- P' ** F *)
+    G |-- embed (ap (T := Fun locals) (fun l v => Q' v l) v ** F |-- Q) -> (* Q' ** F |- Q *)
+    G |-- triple P
+                 (Call f e)
+                 Q.
+**)
+
+Require Import Coq.Strings.String.
+Local Open Scope string_scope.
+
+
+Lemma embed_ltrue
+: forall (P : Prop),
+    P ->
+    |-- @embed Prop SProp _ P.
+Admitted.
+Lemma locals_get_locals_upd
+: forall v val m,
+    locals_get v (locals_upd v val m) = val.
+Admitted.
+Lemma eval_iexpr_iPlus
+: forall a b m,
+    eval_iexpr (iPlus a b) m = eval_iexpr a m + eval_iexpr b m.
+Admitted.
+Lemma eval_iexpr_iVar
+: forall a m,
+    eval_iexpr (iVar a) m = locals_get a m.
+Admitted.
+Lemma eval_iexpr_iConst
+: forall a m,
+    eval_iexpr (iConst a) m = a.
+Admitted.
+
+Axiom pull_embed_hyp
+: forall (P : Prop) (Q R : HProp),
+    (P -> (Q |-- R)) ->
+    Q //\\ embed P |-- R.
+Axiom pull_embed_last_hyp
+: forall (P : Prop) (R : HProp),
+    (P -> |-- R) ->
+    embed P |-- R.
+*)
