examples/Hoare/ImpMetaTheory.v
@@ -1,0 +1,152 @@
+Require Import McExamples.Hoare.ILogic.
+Require Import McExamples.Hoare.Imp.
+
+Module ImpTheory (Import I : ImpLang).
+  Lemma entails_exL
+  : forall (P : value -> locals -> HProp) Q,
+    (forall x, P x |-- Q) ->
+    lexists P |-- Q.
+  Admitted.
+
+  Lemma go_lower
+    : forall (P Q : lprop) (G : SProp),
+      G |-- lforall (fun x : locals => embed (P x |-- Q x)) ->
+      G |-- @embed Prop SProp EmbedOp_Prop_SProp (P |-- Q).
+  Admitted.
+  Lemma go_lower_raw
+    : forall (P Q : lprop),
+      (forall x : locals, P x |-- Q x) ->
+      (P |-- Q).
+  Admitted.
+
+  Lemma embed_ltrue
+    : forall (P : Prop),
+      P ->
+      |-- @embed Prop SProp _ P.
+  Admitted.
+  Lemma locals_get_locals_upd
+    : forall v val m,
+      locals_get v (locals_upd v val m) = val.
+  Admitted.
+  Lemma eval_iexpr_iPlus
+    : forall a b m,
+      eval_iexpr (iPlus a b) m = eval_iexpr a m + eval_iexpr b m.
+  Admitted.
+  Lemma eval_iexpr_iVar
+    : forall a m,
+      eval_iexpr (iVar a) m = locals_get a m.
+  Admitted.
+  Lemma eval_iexpr_iConst
+    : forall a m,
+      eval_iexpr (iConst a) m = a.
+  Admitted.
+
+  Axiom pull_embed_hyp
+    : forall (P : Prop) (Q R : HProp),
+      (P -> (Q |-- R)) ->
+      Q //\\ embed P |-- R.
+  Axiom pull_embed_last_hyp
+    : forall (P : Prop) (R : HProp),
+      (P -> |-- R) ->
+      embed P |-- R.
+
+
+  Theorem Assign_seq_rule
+    : forall G P Q x e c,
+      G |-- triple (Exists v' : value, (fun l =>
+                                          P  (locals_upd x v' l) //\\
+                                             embed (locals_get x l = eval_iexpr e (locals_upd x v' l)))) c Q ->
+      G |-- triple P
+        (Seq (Assign x e) c)
+        Q.
+  Proof.
+    intros. eapply Seq_rule. eapply Assign_rule. eassumption.
+  Qed.
+
+  Theorem Assign_tail_rule
+    : forall G P Q x e,
+      G |-- embed (Exists v' : value, (fun l => 
+                                         P  (locals_upd x v' l) //\\
+                                            embed (locals_get x l = eval_iexpr e (locals_upd x v' l))) |-- Q) ->
+      G |-- triple P (Assign x e) Q.
+  Proof.
+    intros.
+    eapply Conseq_rule. 3: eapply Assign_rule.
+    2: eapply H.
+    admit.
+  Admitted.
+
+(*
+  Theorem Read_seq_rule
+    : forall G (P Q : lprop) x e (v : locals -> value) c,
+      (G |-- embed (P |-- ap (T := Fun locals) (ap (pure PtsTo) (eval_iexpr e)) v ** ltrue)) ->
+      (G |-- triple (Exists v' : value, fun l =>
+                                          P (locals_upd x v' l)
+                                            //\\  embed (locals_get x l = v (locals_upd x v' l))) c Q) ->
+      G |-- triple P (Seq (Read x e) c) Q.
+  Proof.
+    intros. eapply Seq_rule. eapply Read_rule. eapply H. assumption.
+  Qed.
+
+  Theorem Read_tail_rule
+    : forall G (P Q : lprop) x e (v : locals -> value),
+      (G |-- embed (P |-- ap (T := Fun locals) (ap (pure PtsTo) (eval_iexpr e)) v ** ltrue)) ->
+      (G |-- embed (Exists v' : value, (fun l =>
+                                          P (locals_upd x v' l)
+                                            //\\  embed (locals_get x l = v (locals_upd x v' l))) |-- Q)) ->
+      G |-- triple P (Read x e) Q.
+  Proof.
+    intros. eapply Conseq_rule; [ | | eapply Read_rule ].
+    3: eassumption. admit. eassumption.
+  Qed.
+
+  Theorem Write_seq_rule
+    : forall G (P Q R : lprop) p v c,
+      (G |-- embed (P |-- Exists v', ap (T := Fun locals) (ap (pure PtsTo) (eval_iexpr p)) (pure v') ** Q)) ->
+      (G |-- triple (ap (T := Fun locals) (ap (pure PtsTo) (eval_iexpr p)) (eval_iexpr v) ** Q) c R) ->
+      G |-- triple P (Seq (Write p v) c) R.
+  Proof.
+    intros. eapply Seq_rule. eapply Write_rule. eassumption. eassumption.
+  Qed.
+
+  Theorem Write_tail_rule
+    : forall G (P Q R : lprop) p v,
+      G |-- embed (P |-- Exists v', ap (T := Fun locals) (ap (pure PtsTo) (eval_iexpr p)) (pure v') ** Q) ->
+      (G |-- embed ((ap (T := Fun locals) (ap (pure PtsTo) (eval_iexpr p)) (eval_iexpr v) ** Q) |-- R)) ->
+      G |-- triple P (Write p v) R.
+  Proof.
+    intros. eapply Conseq_rule. 3: eapply Write_rule. 2: eassumption. 2: eassumption. admit.
+  Qed.
+*)
+
+  Theorem Skip_seq_rule
+    : forall G P Q c,
+      G |-- triple P c Q ->
+      G |-- triple P (Seq Skip c) Q.
+  Proof.
+    intros. eapply Seq_rule. eapply Skip_rule_refl. eassumption.
+  Qed.
+
+  Definition Skip_tail_rule := Skip_rule.
+
+  Theorem Assert_seq_rule
+    : forall G P Q A c,
+      G |-- embed (P |-- A) ->
+      G |-- triple A c Q ->
+      G |-- triple P (Seq (Assert A) c) Q.
+  Proof.
+    intros. eapply Seq_rule; [ | eapply H0 ].
+    eapply Conseq_rule; [ eassumption | | eapply Assert_rule ].
+    admit.
+  Admitted.
+
+  Theorem Assert_tail_rule
+    : forall G P Q A,
+      G |-- embed (P |-- A) ->
+      G |-- embed (A |-- Q) ->
+      G |-- triple P (Assert A) Q.
+  Proof.
+    intros. eapply Conseq_rule; try eassumption.
+    eapply Assert_rule.
+  Qed.
+End ImpTheory.
