examples/Hoare/ImpSyntax.v
@@ -1,0 +1,682 @@
+Require Import Coq.Bool.Bool.
+Require Import ExtLib.Core.RelDec.
+Require Import ExtLib.Data.String.
+Require Import MirrorCore.TypesI.
+Require Import MirrorCore.ExprI.
+Require Import MirrorCore.ModularTypes.
+Require Import MirrorCore.syms.SymEnv.
+Require Import MirrorCore.syms.SymSum.
+Require Import MirrorCore.Lambda.Expr.
+Require Import MirrorCore.Views.FuncView.
+Require Import McExamples.Hoare.Imp.
+Require Import McExamples.Hoare.ILogicFunc.
+
+Module ImpSyntax (I : ImpLang).
+  (* Types *)
+  Inductive tsym : nat -> Type :=
+  | tyLocals   : tsym 0
+  | tyCmd      : tsym 0
+  | tySProp    : tsym 0
+  | tyHProp    : tsym 0
+  | tyProp     : tsym 0
+  | tyVariable : tsym 0
+  | tyExpr     : tsym 0
+  | tyValue    : tsym 0.
+
+  Definition tsymD (n : nat) (t : tsym n) : type_for_arity n :=
+    match t with
+    | tyLocals => I.locals
+    | tyCmd => I.icmd
+    | tySProp => I.SProp
+    | tyHProp => I.HProp
+    | tyProp => Prop
+    | tyVariable => I.var
+    | tyExpr => I.iexpr
+    | tyValue => I.value
+    end.
+
+  Definition tsym_tag {n} (t : tsym n) : nat :=
+    match t with
+    | tyLocals => 0
+    | tyCmd => 1
+    | tySProp => 2
+    | tyHProp => 3
+    | tyVariable => 4
+    | tyExpr => 5
+    | tyValue => 6
+    | tyProp => 7
+    end.
+
+  Definition tsym_neq : forall n (a b : tsym n),
+      tsym_tag a <> tsym_tag b ->
+      a <> b.
+  Proof.
+    intros. intro.
+    apply H. destruct H0.
+    reflexivity.
+  Defined.
+
+  Definition tsym_dec {n} (a : tsym n) : forall b, {a = b} + {a <> b}.
+  refine
+    match a as a in tsym n return forall b : tsym n, {a = b} + {a <> b} with
+    | tyLocals => fun b =>
+                    match b with
+                    | tyLocals => left eq_refl
+                    | _ => right _
+                    end
+    | tyCmd => fun b =>
+                    match b with
+                    | tyCmd => left eq_refl
+                    | _ => right _
+                    end
+    | tySProp => fun b =>
+                    match b with
+                    | tySProp => left eq_refl
+                    | _ => right _
+                    end
+    | tyHProp => fun b =>
+                    match b with
+                    | tyHProp => left eq_refl
+                    | _ => right _
+                    end
+    | tyProp => fun b =>
+                    match b with
+                    | tyProp => left eq_refl
+                    | _ => right _
+                    end
+    | tyVariable => fun b =>
+                    match b with
+                    | tyVariable => left eq_refl
+                    | _ => right _
+                    end
+    | tyExpr => fun b =>
+                    match b with
+                    | tyExpr => left eq_refl
+                    | _ => right _
+                    end
+    | tyValue => fun b =>
+                    match b with
+                    | tyValue => left eq_refl
+                    | _ => right _
+                    end
+    end; try solve [ intro x ; revert x ; apply tsym_neq ;
+                     clear; compute; congruence ].
+  Defined.
+
+  Definition typ := mtyp tsym.
+
+  Global Instance RType_typ : RType typ := RType_mtyp _ tsymD (@tsym_dec).
+  Global Instance RTypeOk_typ : RTypeOk := RTypeOk_mtyp _ _ _.
+
+  Global Instance Typ2_Fun : @Typ2 typ _ Fun := Typ2_Fun.
+  Global Instance Typ2Ok_Fun : Typ2Ok Typ2_Fun := Typ2Ok_Fun.
+  Global Instance Typ0_Prop : @Typ0 typ _ Prop := Typ0_sym tyProp.
+  Global Instance Typ0Ok_Prop : Typ0Ok Typ0_Prop := Typ0Ok_sym tyProp.
+
+  Global Instance RelDec_eq_typ : RelDec (@eq typ) := RelDec_Rty _.
+  Global Instance RelDec_Correct_eq_typ : RelDec_Correct RelDec_eq_typ :=
+    @RelDec_Correct_Rty _ _ _.
+
+  (* Symbols *)
+  Inductive imp_func :=
+  | pVar (_ : I.var)
+  | pNat (_ : nat)
+  | pLocals_get | pLocals_upd
+  | pEq (_ : typ)
+  | pEval_expri
+  | eVar | eConst | ePlus
+  | natPlus
+  (** Below here isn't really imp functions **)
+  | pAp (_ _ : typ)
+  | pPure (_ : typ)
+  | pUpdate (_ : typ).
+
+  Definition func := (SymEnv.func + imp_func + ilfunc typ)%type.
+
+  Local Notation "! x" := (@tyBase0 tsym x) (at level 0).
+
+  Arguments tyArr {_} _ _.
+
+  Definition typeof_sym_imp (f : imp_func) : option typ :=
+    match f with
+    | pVar _ => Some !tyVariable
+    | pNat _ => Some !tyValue
+    | pLocals_get => Some (tyArr !tyVariable (tyArr !tyLocals !tyValue))
+    | pLocals_upd => Some (tyArr !tyVariable (tyArr !tyValue (tyArr !tyLocals !tyLocals)))
+    | pEq t => Some (tyArr t (tyArr t !tyProp))
+    | pEval_expri => Some (tyArr !tyExpr (tyArr !tyLocals !tyValue))
+    | eVar => Some (tyArr !tyVariable !tyExpr)
+    | eConst => Some (tyArr !tyValue !tyExpr)
+    | ePlus => Some (tyArr !tyExpr (tyArr !tyExpr !tyExpr))
+    | natPlus => Some (tyArr !tyValue (tyArr !tyValue !tyValue))
+    | pAp t u => Some (tyArr (tyArr !tyLocals (tyArr t u)) (tyArr (tyArr !tyLocals t) (tyArr !tyLocals u)))
+    | pPure t => Some (tyArr t (tyArr !tyLocals t))
+    | pUpdate t => Some (tyArr (tyArr !tyLocals !tyLocals)
+                               (tyArr (tyArr !tyLocals t)
+                                      (tyArr !tyLocals t)))
+    end.
+
+  Definition imp_func_eq (a b : imp_func) : option bool :=
+    match a , b with
+    | pVar a , pVar b => Some (a ?[ eq ] b)
+    | pNat a , pNat b => Some (a ?[ eq ] b)
+    | pLocals_get , pLocals_get => Some true
+    | pLocals_upd , pLocals_upd => Some true
+    | pEq a , pEq b => Some (a ?[ Rty ] b)
+    | pEval_expri , pEval_expri => Some true
+    | eVar , eVar => Some true
+    | eConst , eConst => Some true
+    | ePlus , ePlus => Some true
+    | natPlus , natPlus => Some true
+    | pAp t u , pAp t' u' => Some (t ?[ Rty ] t' && u ?[ Rty ] u')%bool
+    | pPure t , pPure t' => Some (t ?[ Rty ] t')
+    | pUpdate t , pUpdate t' => Some (t ?[ Rty ] t')
+    | _ , _ => Some false
+    end.
+
+  Instance RSym_imp_func : SymI.RSym imp_func :=
+  { typeof_sym := typeof_sym_imp
+  ; symD := fun f =>
+    match f as f return match typeof_sym_imp f with
+                        | None => unit
+                        | Some t => typD t
+                        end
+    with
+    | pVar v => v
+    | pNat n => n
+    | pLocals_get => I.locals_get
+    | pLocals_upd => I.locals_upd
+    | pEq t => @eq _
+    | pEval_expri => I.eval_iexpr
+    | eVar => I.iVar
+    | eConst => I.iConst
+    | ePlus => I.iPlus
+    | natPlus => plus
+    | pPure t =>
+      @Applicative.pure (RFun I.locals) (Applicative_Fun _) (typD t)
+    | pAp t u =>
+      @Applicative.ap (RFun I.locals) (Applicative_Fun _) (typD t) (typD u)
+    | pUpdate t => I.update
+    end
+  ; sym_eqb := imp_func_eq
+  }.
+
+  Instance RSymOk_imp_func : SymI.RSymOk RSym_imp_func.
+  constructor.
+  - destruct a; destruct b; simpl; try congruence.
+    Require Import ExtLib.Tactics.Consider.
+    all: match goal with
+         | |- context [ if ?X then _ else _ ] =>
+           consider X; intros; unfold Rty in *; try congruence
+         end.
+    f_equal; tauto.
+    destruct H; congruence.
+  Qed.
+
+  Instance FuncView_ilfunc : FuncView func (ilfunc typ).
+  Admitted.
+
+  Definition tyLProp := tyArr !tyLocals !tyHProp.
+
+  Local Notation "a >> b" := (tyArr a b) (at level 31,right associativity).
+
+  Require Import Coq.Lists.List.
+  (** TODO: Note that this needs to be extensible! **)
+  Definition fs : @SymEnv.functions typ _ :=
+    SymEnv.from_list
+      (@SymEnv.F typ _ (tyArr tyLProp (tyArr !tyCmd (tyArr tyLProp !tySProp)))
+                 I.triple ::
+       @SymEnv.F typ _ (tyArr !tyCmd (tyArr !tyCmd !tyCmd)) I.Seq ::
+       @SymEnv.F typ _ (tyArr !tyVariable (tyArr !tyExpr !tyCmd)) I.Assign ::
+       @SymEnv.F typ _ !tyCmd I.Skip ::
+       @SymEnv.F typ _ (tyArr tyLProp !tyCmd) I.Assert ::
+       @SymEnv.F typ _ (tyArr !tyExpr (tyArr !tyCmd (tyArr !tyCmd !tyCmd))) I.If ::
+       @SymEnv.F typ _ (tyArr !tyValue !tyValue) S ::
+                 (*     @SymEnv.F typ _ (tyArr tyVariable (tyArr tyExpr tyCmd))
+               (I.Read) ::
+     @SymEnv.F typ _ (tyArr tyExpr (tyArr tyExpr tyCmd))
+               (Write) :: *)
+                 (*     @SymEnv.F typ _ (tyArr tyValue (tyArr tyValue tyHProp))
+               (PtsTo) :: *)
+                 (* @SymEnv.F typ _ (tyArr tyValue tyProp) *)
+                 (*           (Even.even) :: *)
+                 (* @SymEnv.F typ _ (tyArr tyValue tyProp) *)
+                 (*           (Even.odd) :: *)
+                 (*
+     @SymEnv.F typ _ (tyVariable >> (tyValue >> tyLProp) >> (tyValue >> tyLProp) >> tySProp)
+               (function_spec) ::
+                  *)
+       nil).
+
+  Definition lops : @logic_ops typ _ :=
+    fun t : typ =>
+      match t as t
+             return loption (ILogic.ILogicOps@{Urefl Urefl} (TypesI.typD t))
+      with
+      | tyArr a b =>
+        match a , b with
+        | tyBase0 a , tyBase0 b =>
+          match a as a in tsym na , b as b in tsym nb
+                return match na as na , nb as nb
+                             return tsym na -> tsym nb -> Type
+                       with
+                       | 0 , 0 => fun a b =>
+                                    loption (ILogic.ILogicOps@{Urefl Urefl} (tsymD 0 a -> tsymD _ b))
+                       | _ , _ => fun _ _ => unit
+                       end a b
+          with
+          | tyLocals , tyHProp => lSome (I.ILogicOps_lprop)
+          | _ , _ => lNone
+          end
+        | _ , _ => lNone
+        end
+      | tyBase0 l =>
+        match l as l in tsym 0 return loption (ILogic.ILogicOps@{Urefl Urefl} (tsymD _ l)) with
+        | tyProp => lSome _
+        | tyHProp => lSome _
+        | tySProp => lSome _
+        | _ => lNone
+        end
+      | tyBase1 _ _ => lNone
+      | tyBase2 _ _ _ => lNone
+      | tyApp _ _ => lNone
+      end.
+
+  Definition eops : embed_ops _ :=
+    fun t u =>
+      match t as t
+            return loption
+                     (ILogic.EmbedOp (TypesI.typD t) (TypesI.typD u))
+      with
+      | tyBase0 t =>
+        match t as t in tsym 0
+              return loption (ILogic.EmbedOp (tsymD _ t) (TypesI.typD u))
+        with
+        | tyProp =>
+          match u with
+          | tyBase0 u =>
+            match u as u in tsym 0
+                  return loption (ILogic.EmbedOp Prop (tsymD 0 u))
+            with
+            | tyHProp => lSome I.EmbedOp_Prop_HProp
+            | tySProp => lSome I.EmbedOp_Prop_SProp
+            | _ => lNone
+            end
+          | tyArr a b =>
+            match a as a , b as b
+                  return loption (ILogic.EmbedOp Prop (TypesI.typD a -> TypesI.typD b))
+            with
+            | tyBase0 a , tyBase0 b =>
+              match a as a in tsym na , b as b in tsym nb
+                    return match na as na , nb as nb
+                                 return tsym na -> tsym nb -> Type
+                           with
+                           | 0 , 0 => fun a b => loption (ILogic.EmbedOp Prop (tsymD _ a -> tsymD _ b))
+                           | _ , _ => fun _ _ => unit
+                           end a b
+              with
+              | tyLocals , tyHProp => lSome (@ILogic.EmbedOp_Fun _ _ I.EmbedOp_Prop_HProp _)
+              | _ , _ => lNone
+              end
+            | _ , _ => lNone
+            end
+          | _ => lNone
+          end
+        | tyHProp =>
+          match u with
+          | tyArr a b =>
+            match a as a , b as b
+                  return loption (ILogic.EmbedOp I.HProp (TypesI.typD a -> TypesI.typD b))
+            with
+            | tyBase0 a , tyBase0 b =>
+              match a as a in tsym na , b as b in tsym nb
+                    return match na as na , nb as nb
+                                 return tsym na -> tsym nb -> Type
+                           with
+                           | 0 , 0 => fun a b => loption (ILogic.EmbedOp I.HProp (tsymD _ a -> tsymD _ b))
+                           | _ , _ => fun _ _ => unit
+                           end a b
+              with
+              | tyLocals , tyHProp => lSome I.EmbedOp_HProp_lprop
+              | _ , _ => lNone
+              end
+            | _ , _ => lNone
+            end
+          | _ => lNone
+          end
+        | _ => lNone
+        end
+      | _ => lNone
+      end.
+
+  Local Instance RSym_ilfunc : SymI.RSym (ilfunc typ) :=
+    @ILogicFunc.RSym_ilfunc typ _ _ lops eops _ _.
+
+  Definition RS : SymI.RSym func :=
+    SymSum.RSym_sum (SymSum.RSym_sum (SymEnv.RSym_func fs) _) _.
+  Local Existing Instance RS.
+
+  Instance RSOk : SymI.RSymOk RS.
+  eapply RSymOk_sum; eauto with typeclass_instances.
+  eapply RSymOk_sum; eauto with typeclass_instances.
+  Defined.
+
+  Definition Expr_expr : ExprI.Expr _ (expr typ func) := @Expr_expr typ func _ _ _.
+  Local Existing Instance Expr_expr.
+
+  Definition ExprOk_expr : ExprI.ExprOk Expr_expr := ExprOk_expr.
+  Existing Instance ExprOk_expr.
+
+(*
+Definition subst : Type :=
+  FMapSubst.SUBST.raw (expr typ func).
+Definition SS : SubstI.Subst subst (expr typ func) :=
+  @FMapSubst.SUBST.Subst_subst _.
+Definition SU : SubstI.SubstUpdate subst (expr typ func) :=
+  @FMapSubst.SUBST.SubstUpdate_subst _ _.
+Definition SO := FMapSubst.SUBST.SubstOk_subst.
+
+Local Existing Instance SS.
+Local Existing Instance SU.
+Local Existing Instance SO.
+*)
+
+
+  Instance RelDec_eq_imp_func : RelDec (@eq imp_func) :=
+  { rel_dec := fun a b =>
+    match a , b with
+    | pVar a , pVar b => a ?[ eq ] b
+    | pNat a , pNat b => a ?[ eq ] b
+    | pLocals_get , pLocals_get => true
+    | pLocals_upd , pLocals_upd => true
+    | pEq a , pEq b => a ?[ eq ] b
+    | pEval_expri , pEval_expri => true
+    | eVar , eVar
+    | eConst , eConst => true
+    | pAp a a' , pAp b b' => (a ?[ eq ] b) && (a' ?[ eq ] b')
+    | pPure a , pPure b => a ?[ eq ] b
+    | pUpdate a , pUpdate b => a ?[ eq ] b
+    | _ , _ => false
+    end
+  }.
+
+
+  Instance RelDec_eq_func : RelDec (@eq func) :=
+  { rel_dec := fun a b =>
+    match a , b with
+    | inl (inl a) , inl (inl b) => a ?[ eq ] b
+    | inl (inr a) , inl (inr b) => a ?[ eq ] b
+    | inr a , inr b => a ?[ eq ] b
+    | _ , _ => false
+    end
+  }.
+
+  Definition RelDec_eq_expr : RelDec (@eq (expr typ func)) :=
+    @RelDec_eq_expr typ func _ _.
+
+
+  Definition fTriple : expr typ func := Inj (inl (inl 1%positive)).
+  Definition fSeq : expr typ func := Inj (inl (inl 2%positive)).
+  Definition fAssign : expr typ func := Inj (inl (inl 3%positive)).
+  Definition fSkip : expr typ func := Inj (inl (inl 6%positive)).
+  Definition fAssert : expr typ func := Inj (inl (inl 7%positive)).
+(*
+  Definition fRead : expr typ func := Inj (inl (inl 4%positive)).
+  Definition fWrite : expr typ func := Inj (inl (inl 5%positive)).
+  Definition fPtsTo : expr typ func := Inj (inl (inl 8%positive)).
+*)
+  Definition fEven : expr typ func := Inj (inl (inl 9%positive)).
+  Definition fOdd : expr typ func := Inj (inl (inl 10%positive)).
+  Definition fS : expr typ func := Inj (inl (inl 11%positive)).
+
+
+  Definition feVar : expr typ func := Inj (inl (inr eVar)).
+  Definition feConst : expr typ func := Inj (inl (inr eConst)).
+  Definition fePlus : expr typ func := Inj (inl (inr ePlus)).
+  Definition fPlus : expr typ func := Inj (inl (inr natPlus)).
+
+  Definition fVar (v : I.var) : expr typ func := Inj (inl (inr (pVar v))).
+  Definition fConst (c : I.value) : expr typ func := Inj (inl (inr (pNat c))).
+  Definition fAp (t u : typ) : expr typ func := Inj (inl (inr (pAp t u))).
+  Definition fPure (t : typ) : expr typ func := Inj (inl (inr (pPure t))).
+  Definition flocals_get : expr typ func := Inj (inl (inr pLocals_get)).
+  Definition flocals_upd : expr typ func := Inj (inl (inr pLocals_upd)).
+  Definition fupdate t : expr typ func := Inj (inl (inr (pUpdate t))).
+  Definition feval_iexpr : expr typ func := Inj (inl (inr pEval_expri)).
+  Definition fEq (t : typ) : expr typ func := Inj (inl (inr (pEq t))).
+
+  Definition mkTriple (P c Q : expr typ func) : expr typ func :=
+    App (App (App fTriple P) c) Q.
+  Definition mkSeq (a b : expr typ func) : expr typ func :=
+    App (App fSeq a) b.
+  Definition mkAssign (a b : expr typ func) : expr typ func :=
+    App (App fAssign a) b.
+(*
+  Definition mkRead (a b : expr typ func) : expr typ func :=
+    App (App fRead a) b.
+  Definition mkWrite (a b : expr typ func) : expr typ func :=
+    App (App fWrite a) b.
+*)
+  Definition mkSkip : expr typ func := fSkip.
+
+  Definition lex (l t : typ) (e : expr typ func) : expr typ func :=
+    App (Inj (inr (ilf_exists t l))) (Abs t e).
+
+(*Definition lstar (l : typ) (e e' : expr typ func) : expr typ func :=
+  App (App (fStar l)  e) e'.
+Definition lemp (l : typ) : expr typ func := fEmp l.
+*)
+  Definition land (l : typ) (e e' : expr typ func) : expr typ func :=
+    App (App (Inj (inr (ilf_and l))) e) e'.
+  Definition ltrue (l : typ) : expr typ func :=
+    Inj (inr (ilf_true l)).
+  Definition lentails (l : typ) (e e' : expr typ func) : expr typ func :=
+    App (App (Inj (inr (ilf_entails l))) e) e'.
+  Definition lor (l : typ) (e e' : expr typ func) : expr typ func :=
+    App (App (Inj (inr (ilf_or l))) e) e'.
+  Definition lembed (t f : typ) (e : expr typ func) : expr typ func :=
+    App (Inj (inr (ilf_embed f t))) e.
+(*
+  Definition lPtsTo (a b : expr typ func) : expr typ func :=
+    App (App fPtsTo a) b.
+*)
+
+  Definition lap (t u : typ) (a b : expr typ func) : expr typ func :=
+    App (App (fAp t u) a) b.
+  Definition lpure (t : typ) (a : expr typ func) : expr typ func :=
+    App (fPure t) a.
+  Definition lupdate (t : typ) (a b : expr typ func) : expr typ func :=
+    App (App (fupdate t) a) b.
+
+(*
+(** Testing function **)
+Definition test_lemma :=
+  @lemmaD typ (expr typ func) RType_typ Expr_expr (expr typ func)
+          (fun tus tvs e => exprD' tus tvs tyProp e)
+          Typ0_Prop nil nil.
+*)
+  (** Reification *)
+  Require Import MirrorCore.Reify.Reify.
+
+  Local Notation "x @ y" := (@RApp x y) (only parsing, at level 30).
+  Local Notation "'!!' x" := (@RExact _ x) (only parsing, at level 25).
+  Local Notation "'?' n" := (@RGet n RIgnore) (only parsing, at level 25).
+  Local Notation "'?!' n" := (@RGet n RConst) (only parsing, at level 25).
+  Local Notation "'#'" := RIgnore (only parsing, at level 0).
+
+  Reify Declare Patterns patterns_imp_typ : typ.
+
+  Reify Declare Typed Table term_table : BinNums.positive => typ.
+
+  Reify Declare Syntax reify_imp_typ :=
+    Patterns.CPatterns patterns_imp_typ.
+
+  Reify Declare Patterns patterns_ilogic_func : ilfunc typ.
+  Reify Declare Patterns patterns_imp_func : imp_func.
+  Reify Declare Patterns patterns_imp : expr typ func.
+
+  Definition mkLogic (x : ilfunc typ) : expr typ func :=
+    ExprCore.Inj (inr x).
+  Definition mkExt (x : BinNums.positive) : expr typ func :=
+    ExprCore.Inj (inl (inl x)).
+
+
+  Reify Declare Syntax reify_imp :=
+    Patterns.CFirst (   Patterns.CVar (@ExprCore.Var typ func)
+                     :: Patterns.CMap mkLogic patterns_ilogic_func
+                     :: Patterns.CPatterns patterns_imp
+                     :: Patterns.CApp (@ExprCore.App typ func)
+                     :: Patterns.CAbs reify_imp_typ (@ExprCore.Abs typ func)
+                     :: Patterns.CMap mkExt (Patterns.CTypedTable reify_imp_typ term_table)
+                     :: nil).
+
+  (** BEGIN LOGIC REIFY **)
+  (** TODO: It would be nice to be able to put these elsewhere *)
+  Reify Pattern patterns_ilogic_func += (!! @ILogic.lentails @ ?0 @ #) =>
+    fun (x : function reify_imp_typ) => @ILogicFunc.ilf_entails typ x.
+  Reify Pattern patterns_ilogic_func += (!! @ILogic.ltrue @ ?0 @ #) =>
+    fun (x : function reify_imp_typ) => @ILogicFunc.ilf_true typ x.
+  Reify Pattern patterns_ilogic_func += (!! @ILogic.lfalse @ ?0 @ #) =>
+    fun (x : function reify_imp_typ) => @ILogicFunc.ilf_false typ x.
+  Reify Pattern patterns_ilogic_func += (!! @ILogic.land @ ?0 @ #) =>
+    fun (x : function reify_imp_typ) => @ILogicFunc.ilf_and typ x.
+  Reify Pattern patterns_ilogic_func += (!! @ILogic.lor @ ?0 @ #) =>
+    fun (x : function reify_imp_typ) => @ILogicFunc.ilf_or typ x.
+  Reify Pattern patterns_ilogic_func += (!! @ILogic.limpl @ ?0 @ #) =>
+    fun (x : function reify_imp_typ) => @ILogicFunc.ilf_impl typ x.
+  Reify Pattern patterns_ilogic_func += (!! @ILogic.lexists @ ?0 @ # @ ?1) =>
+    fun (x y : function reify_imp_typ) => @ILogicFunc.ilf_exists typ y x.
+  Reify Pattern patterns_ilogic_func += (!! @ILogic.lforall @ ?0 @ # @ ?1) =>
+    fun (x y : function reify_imp_typ) => @ILogicFunc.ilf_forall typ y x.
+
+  (** Embedding Operators **)
+  Reify Pattern patterns_ilogic_func += (!! @ILogic.embed @ ?0 @ ?1 @ #) =>
+    fun (x y : function reify_imp_typ) => ILogicFunc.ilf_embed x y.
+
+  (** Special cases for Coq's primitives **)
+  Reify Pattern patterns_ilogic_func += (!!True) => ILogicFunc.ilf_true !tyProp.
+  Reify Pattern patterns_ilogic_func += (!!False) => ILogicFunc.ilf_false !tyProp.
+  Reify Pattern patterns_ilogic_func += (!!and) => ILogicFunc.ilf_and !tyProp.
+  Reify Pattern patterns_ilogic_func += (!! or) => ILogicFunc.ilf_or !tyProp.
+
+  Reify Pattern patterns_imp += (RPi (?0) (?1)) =>
+    fun (x : function reify_imp_typ) (y : function reify_imp) =>
+      ExprCore.App (mkLogic (@ILogicFunc.ilf_forall typ x !tyProp ))
+                   (@ExprCore.Abs typ func x y).
+  Reify Pattern patterns_imp += (RImpl (?0) (?1)) =>
+    fun (x y : function reify_imp) =>
+      ExprCore.App (ExprCore.App (mkLogic (@ILogicFunc.ilf_impl typ !tyProp)) x) y.
+  (** END LOGIC REIFY **)
+
+
+
+  (** BEGIN TYPE REIFY **)
+  Reify Pattern patterns_imp_typ += (@RImpl (?0) (?1)) =>
+    fun (a b : function reify_imp_typ) => tyArr a b.
+  Reify Pattern patterns_imp_typ += (!! I.locals)  => !tyLocals.
+  Reify Pattern patterns_imp_typ += (!! I.lprop)  => tyArr !tyLocals !tyHProp.
+  Reify Pattern patterns_imp_typ += (!! I.icmd) => !tyCmd.
+  Reify Pattern patterns_imp_typ += (!! I.SProp) => !tySProp.
+  Reify Pattern patterns_imp_typ += (!! I.HProp) => !tyHProp.
+  Reify Pattern patterns_imp_typ += (!! Prop) => !tyProp.
+  Reify Pattern patterns_imp_typ += (!! I.var) => !tyVariable.
+  Reify Pattern patterns_imp_typ += (!! I.iexpr) => !tyExpr.
+  Reify Pattern patterns_imp_typ += (!! nat)  => !tyValue.
+  Reify Pattern patterns_imp_typ += (!! I.value)  => !tyValue.
+  Reify Pattern patterns_imp_typ += (!! Fun @ ?0 @ ?1) =>
+    fun (a b : function reify_imp_typ) => tyArr a b.
+  Reify Pattern patterns_imp_typ += (!! PreFun.Fun @ ?0 @ ?1) =>
+    fun (a b : function reify_imp_typ) => tyArr a b.
+
+
+  (** BEGIN TERM REIFY **)
+  (** Reify imp_func **)
+  Reify Pattern patterns_imp_func += (RHasType var (?!0)) =>
+    fun (x : id I.var) => pVar x.
+  Reify Pattern patterns_imp_func += (RHasType String.string (?!0)) =>
+    fun (x : id I.var) => pVar x.
+  Reify Pattern patterns_imp_func += (RHasType nat (?!0)) =>
+    fun (x : id nat) => pNat x.
+  Reify Pattern patterns_imp_func += (!! (@eq) @ ?0) =>
+    fun (x : function reify_imp_typ) => pEq x.
+
+  (** Expressions **)
+  Reify Pattern patterns_imp_func += (!! I.iConst) => eConst.
+  Reify Pattern patterns_imp_func += (!! I.iVar) => eVar.
+  Reify Pattern patterns_imp_func += (!! I.iPlus) => ePlus.
+
+  (** Arith **)
+  Reify Pattern patterns_imp_func += (!! plus) => natPlus.
+
+  (** Applicative **)
+  Reify Pattern patterns_imp_func += (!! @Applicative.ap @ !! (PreFun.Fun I.locals) @ # @ ?0 @ ?1) =>
+    fun (x y : function reify_imp_typ) => fAp x y.
+  Reify Pattern patterns_imp += (!! @Applicative.pure @ !! (PreFun.Fun I.locals) @ # @ ?0) =>
+    fun (x : function reify_imp_typ) => fPure x.
+
+(*
+  (** Commands **)
+  Reify Pattern patterns_imp_func += (!! I.Skip) => fSkip.
+  Reify Pattern patterns_imp += (!! I.Seq) => fSeq.
+  Reify Pattern patterns_imp += (!! I.Assign) => fAssign.
+  Reify Pattern patterns_imp += (!! I.Assert) => fAssert.
+  Reify Pattern patterns_imp += (!! I.If) => fIf.
+
+  (** Program Logic **)
+Reify Pattern patterns_imp += (!! triple) => fTriple.
+Reify Pattern patterns_imp += (!! eval_iexpr) => feval_iexpr.
+Reify Pattern patterns_imp += (!! locals_get) => flocals_get.
+Reify Pattern patterns_imp += (!! locals_upd) => flocals_upd.
+
+Reify Pattern patterns_imp += (!! PtsTo) => fPtsTo.
+*)
+
+  (** Table Entries **)
+  Local Notation "a >> b" := (tyArr a b) (at level 31,right associativity).
+
+  Print fs.
+
+  Reify Seed Typed Table term_table += 1 =>
+    [[ (tyLProp >> !tyCmd >> tyLProp >> !tySProp) , I.triple ]].
+  Reify Seed Typed Table term_table += 2 =>
+    [[ (!tyCmd >> !tyCmd >> !tyCmd) , I.Seq ]].
+  Reify Seed Typed Table term_table += 3 =>
+    [[ (!tyVariable >> !tyExpr >> !tyCmd) , I.Assign ]].
+  Reify Seed Typed Table term_table += 4 => [[ !tyCmd , I.Skip ]].
+  Reify Seed Typed Table term_table += 5 => [[ (tyLProp >> !tyCmd) , I.Assert ]].
+  Reify Seed Typed Table term_table += 6 => [[ (!tyExpr >> !tyCmd >> !tyCmd >> !tyCmd) , I.If ]].
+(*
+  Reify Seed Typed Table term_table += 4 =>
+    [[ (tyVariable >> tyExpr >> tyCmd) , Read ].
+  Reify Seed Typed Table term_table += 5 => [ (tyExpr >> tyExpr >> tyCmd) , Write ].
+
+  Reify Seed Typed Table term_table += 7 => [ (tyNat >> tyNat >> tyHProp) , PtsTo ].
+  Reify Seed Typed Table term_table += 8 => [ (tyNat >> tyProp) , Even.even ].
+  Reify Seed Typed Table term_table += 9 => [ (tyNat >> tyProp) , Even.odd ].
+  Reify Seed Typed Table term_table += 10 => [ tyNat , O ].
+  Reify Seed Typed Table term_table += 11 => [ (tyNat >> tyNat) , S ].
+*)
+
+  Definition elem_ctor : forall x : typ, (typD x) -> @SymEnv.function _ _ :=
+    @SymEnv.F _ _.
+
+  Ltac reify_imp e :=
+    let k fs e :=
+        pose e in
+    reify_expr reify_imp k
+               [[ (fun (y : @mk_dvar_map _ _ _ _ term_table elem_ctor) => True) ]]
+               [[ e ]].
+
+  Reify Pattern patterns_imp += (!! S) => (fS).
+
+  Goal True.
+    reify_imp I.Skip.
+    reify_imp (ILogic.lentails True True).
+    reify_imp ((True -> False) -> True).
+    reify_imp (forall G P Q, ILogic.lentails G (I.triple P I.Skip Q)).
+    Set Printing All.
+    exact I.
+  Defined.
+
+
+End ImpSyntax.
