examples/Hoare/LogicTac.v
@@ -1,0 +1,169 @@
+Require Import MirrorCore.TypesI.
+Require Import MirrorCore.SymI.
+Require Import MirrorCore.Views.FuncView.
+Require Import MirrorCore.Views.Ptrns.
+Require Import MirrorCore.RTac.RTac.
+Require Import MirrorCore.Lambda.Expr.
+Require Import MirrorCore.Lambda.Ptrns.
+Require Import MirrorCore.Lambda.RedAll.
+Require Import MirrorCore.Lambda.ExprVariables.
+Require Import MirrorCore.Lambda.Rtac.
+Require Import McExamples.Hoare.Imp.
+Require Import McExamples.Hoare.ILogicFunc.
+
+Section parametric.
+  Context {typ func : Type}.
+  Context {RType_typ : RType typ}.
+  Context {RTypeOk_typ : RTypeOk}.
+  Context {Typ2_RFun : Typ2 _ RFun}.
+  Context {Typ2Ok_RFun : Typ2Ok Typ2_RFun}.
+  Context {Typ0_Prop : Typ0 _ Prop}.
+  Context {Typ0Ok_Prop : Typ0Ok Typ0_Prop}.
+  Context {RSym_func : RSym func}.
+  Context {RSymOk_func : RSymOk RSym_func}.
+
+  Context {FV : FuncView func (ilfunc typ)}.
+  Variable ilo : @logic_ops  _ _.
+  Variable eo : @embed_ops  _ _.
+  Context {FVO : FuncViewOk FV RSym_func (RSym_ilfunc (RelDec_eq_typ) ilo eo _ _) }.
+
+  Definition bin_op {T U V W} (f : T -> U -> V -> W)
+             (t : ptrn func T) (l : ptrn (expr typ func) U) (r : ptrn (expr typ func) V)
+  : ptrn (expr typ func) W :=
+    appl (appl (inj t) (pmap (fun t x => (x,t)) l))
+         (pmap (fun v tx => let '(t,x) := tx in f t x v) r).
+
+  Definition ptrn_ok_bin_op {T U V W} f t l r :
+    ptrn_ok t -> ptrn_ok l -> ptrn_ok r -> ptrn_ok (@bin_op T U V W f t l r).
+  Proof. Admitted.
+
+  Definition ptrn_entails {T U V}
+             (t : ptrn typ V)
+             (a : ptrn (expr typ func) (V -> T))
+             (b : ptrn (expr typ func) (T -> U))
+  : ptrn (expr typ func) U :=
+    appl (appl (inj (ptrn_view _ (fptrn_lentails t))) a) b.
+
+  Instance ptrn_entails_ok {T U V}
+  : forall t a b, ptrn_ok t -> ptrn_ok a -> ptrn_ok b ->
+                  ptrn_ok (@ptrn_entails T U V t a b).
+  Proof.
+    intros.
+    unfold ptrn_entails.
+    repeat first [ simple eapply ptrn_ok_appl
+                 | simple eapply ptrn_ok_inj
+                 | simple eapply ptrn_view_ok
+                 | simple apply fptrn_lentails_ok ]; eauto.
+  Qed.
+
+  Definition intro_ptrn_all : ptrn (expr typ func) (OpenAs typ (expr typ func)) :=
+    por
+      (appl (inj (ptrn_view _ (fptrn_lforall get (fun t => pmap (fun _ => t) ignore))))
+            (pmap (fun body t => AsAl t (fun arg => Red.beta (lift 0 1 (App body arg)))) get))
+      (ptrn_entails get (pmap (fun G t => (G,t)) get)
+                    (appl (inj (ptrn_view _ (fptrn_lforall get (fun t => pmap (fun _ => t) ignore))))
+                          (pmap (fun body t Gt =>
+                                   let '(G,l) := Gt in
+                                   AsAl t (fun arg =>
+                                             App (App (Inj (f_insert (ilf_forall t l))) (lift 0 1 G))
+                                                 (Red.beta (lift 0 1 (App body arg))))) get))).
+
+  Definition intro_ptrn_hyp : ptrn (expr typ func) (OpenAs typ (expr typ func)) :=
+    bin_op (fun _ P Q => AsHy P Q)
+           (ptrn_view _ (fptrn_limpl ignore)) get get.
+
+  Ltac solve_ok :=
+    repeat first [ simple eapply ptrn_ok_appl
+                 | simple eapply ptrn_ok_inj
+                 | simple eapply ptrn_ok_pmap
+                 | simple eapply ptrn_ok_ignore
+                 | simple eapply ptrn_ok_get
+                 | simple eapply ptrn_view_ok
+                 | simple eapply fptrn_lforall_ok; intros
+                 | simple eapply ptrn_entails_ok ].
+
+  Local Existing Instance RSym_ilfunc.
+  Local Existing Instance RSym_func.
+  Local Existing Instance RType_typ.
+
+  Require Import ExtLib.Tactics.
+  Require Import MirrorCore.Util.Forwardy.
+
+  Lemma exprD'_App_both_cases : forall tus tvs tx ty f x fD xD,
+      exprD' tus tvs (typ2 tx ty) f = Some fD ->
+      exprD' tus tvs tx x = Some xD ->
+      exprD' tus tvs ty (App f x) = Some (AbsAppI.exprT_App fD xD).
+  Proof.
+    intros. autorewrite with exprD_rw.
+    erewrite ExprTac.exprD_typeof_Some by eassumption.
+    rewrite H. rewrite H0.
+    reflexivity.
+  Qed.
+
+  Ltac solve_stuff :=
+    try lazymatch goal with
+  | |- ptrn_ok _ => solve_ok
+  | |- _ =>
+    match goal with
+    | H : Succeeds _ _ _ |- _ =>
+      first [ simple eapply Succeeds_appl in H; [ forward_reason; subst; solve_stuff | clear H; solve_ok | clear H; solve_ok ]
+            | simple eapply Succeeds_pmap in H; [ forward_reason; subst; solve_stuff | clear H; solve_ok ]
+            | simple eapply Succeeds_get in H; subst; solve_stuff
+            | simple eapply Succeeds_inj in H; [ forward_reason; subst; solve_stuff | clear H; solve_ok ]
+            | (eapply Succeeds_ptrn_view in H;
+               [ | solve [ eauto with typeclass_instances ] | clear H ]); [ forward_reason; subst; solve_stuff | ] ]
+    end
+  end.
+
+  Theorem intro_ptrn_all_sound : open_ptrn_sound intro_ptrn_all.
+  Proof.
+    red. intros.
+    unfold intro_ptrn_all in H.
+    eapply Succeeds_por in H; solve_ok.
+    destruct H.
+    - solve_stuff.
+      eapply (@s_elim _ _ _ _ _ (@SucceedsE_fptrn_lforall _ _ _ _ _ _ _ _)) in H1.
+      simpl in H1.
+      forward_reason. subst.
+      solve_stuff.
+      + clear H x1.
+        Opaque Red.beta.
+        unfold Ctx.propD, exprD'_typ0. simpl. intros.
+        forwardy.
+        inv_all. subst.
+        unfold symAs in H. simpl in H.
+        destruct (ilo x2) eqn:?; try congruence.
+        forwardy. inv_all. subst.
+        generalize y. intro. clear H.
+        eapply typ2_inj in y.
+        unfold Rty in y. destruct y; subst.
+        generalize (Red.beta_sound tus (tvs ++ x4 :: nil) (lift 0 1 (App x3 e')) (typ0 (F:=Prop))).
+        simpl lift.
+        (*
+      erewrite exprD'_App_both_cases.
+      4: eassumption.
+         *)
+        admit.
+        eassumption.
+      + solve_ok.
+    - admit.
+  Admitted.
+
+  Definition INTRO_all : rtac typ (expr typ func) :=
+    INTRO_ptrn intro_ptrn_all.
+
+  Let Expr_expr := @Expr_expr _ _ RType_typ _ RSym_func.
+  Local Existing Instance Expr_expr.
+  Let ExprOk_expr : ExprOk Expr_expr := @ExprOk_expr _ _ RType_typ _ RSym_func _ _ _.
+  Local Existing Instance ExprOk_expr.
+
+  Instance RtacSound_INTRO_all : RtacSound INTRO_all.
+  Proof.
+    unfold INTRO_all.
+    unfold Expr_expr.
+    constructor.
+    eapply INTRO_ptrn_sound; eauto.
+    - admit.
+    - eapply intro_ptrn_all_sound.
+  Admitted.
+End parametric.
