examples/Hoare/Verify.v
@@ -1,0 +1,754 @@
+Require Import Coq.Strings.String.
+Require Import MirrorCore.RTac.RTac.
+(*Require Import MirrorCharge.Imp.Goal.*)
+Require Import MirrorCore.RTac.RTac.
+Require Import MirrorCore.Lambda.Rtac.
+Require Import McExamples.Hoare.Imp.
+(*Require Import MirrorCharge.Imp.SymEvalLemmas.*)
+(*Require MirrorCharge.Imp.STacCancel. *)
+Require Import McExamples.Hoare.ImpSyntax.
+Require Import McExamples.Hoare.ImpMetaTheory.
+Require Import McExamples.Hoare.LogicTac.
+(*Require Import MirrorCharge.Imp.RTacTauto. *)
+
+(*
+Local Existing Instance SS.
+Local Existing Instance SU.
+Local Existing Instance RSym_ilfunc.
+Local Existing Instance RS.
+Local Existing Instance RSOk.
+Local Existing Instance Expr_expr.
+Local Existing Instance ExprOk_expr.
+*)
+(*
+Definition runTacK (tac : imp_tacK) : imp_tac :=
+  fun a b c d e f g => tac a b c d e f (GGoal g).
+*)
+
+
+(*
+Fixpoint THENS (ls : list (rtac typ (expr typ func))) : imp_tac :=
+  match ls with
+    | nil => IDTAC
+    | l :: ls => THEN l (runOnGoals (THENS ls))
+  end.
+*)
+(*
+Definition side_solver : imp_tac :=
+  THENS (TRY (THENS (EAPPLY go_lower_lemma ::
+                            INTRO_All ::
+                            BETA_REDUCE :: nil)) ::
+             TRY (EAPPLY embed_ltrue_lemma) ::
+             SIMPLIFY ::
+             STacCancel.stac_cancel ::
+             SIMPLIFY :: tauto_tac :: nil).
+*)
+
+Module ImpVerify (I : ImpLang).
+  Module Import Syntax := ImpSyntax I.
+  Module Import MetaTheory := ImpTheory I.
+  Definition imp_tac := rtac typ (expr typ func).
+  Definition imp_tacK := rtacK typ (expr typ func).
+
+  Definition ON_ENTAILMENT (yes no : imp_tac) : imp_tac :=
+    yes.
+  Arguments ON_ENTAILMENT _%rtac _%rtac _ _ _ _ _ _ _.
+
+  Local Open Scope rtac_scope.
+
+  Reify BuildLemma < reify_imp_typ reify_imp reify_imp >
+    embed_ltrue_lemma : embed_ltrue.
+  Reify BuildLemma < reify_imp_typ reify_imp reify_imp >
+    entails_exL_lemma : entails_exL.
+  Reify BuildLemma < reify_imp_typ reify_imp reify_imp >
+    go_lower_raw_lemma : go_lower_raw.
+  Reify BuildLemma < reify_imp_typ reify_imp reify_imp >
+    pull_embed_hyp_lemma : pull_embed_hyp.
+  Reify BuildLemma < reify_imp_typ reify_imp reify_imp >
+    pull_embed_last_lemma : pull_embed_last_hyp.
+
+  Definition INTRO_All   : imp_tac := INTRO_all.
+  Axiom INTRO_Hyp   : imp_tac.
+  Axiom BETA_REDUCE : imp_tac.
+  Axiom SIMPLIFY    : imp_tac.
+
+  Local Existing Instance RType_typ.
+  Local Existing Instance RTypeOk_typ.
+  Local Existing Instance Expr_expr.
+  Local Existing Instance ExprOk_expr.
+  Local Existing Instance Typ2_Fun.
+  Local Existing Instance Typ2Ok_Fun.
+  Local Existing Instance Typ0_Prop.
+  Local Existing Instance Typ0Ok_Prop.
+  Local Existing Instance RS.
+  Local Existing Instance RSOk.
+
+  Definition ON_ALL : rtac typ (expr typ func) -> rtacK typ (expr typ func) :=
+    @ON_ALL _ _ _ _.
+  Definition ON_ALL' : imp_tac -> rtacK typ (expr typ func) := ON_ALL.
+  Coercion ON_ALL : rtac >-> rtacK.
+  Coercion ON_ALL' : imp_tac >-> rtacK.
+
+  Definition entailment_tac : imp_tac :=
+    ON_ENTAILMENT
+      (TRY (EAPPLY embed_ltrue_lemma) ;;
+       TRY (EAPPLY entails_exL_lemma ;;
+            INTRO_All ;;
+            BETA_REDUCE) ;;
+       TRY (EAPPLY go_lower_raw_lemma ;;
+            BETA_REDUCE ;; INTRO_All ;; BETA_REDUCE) ;;
+       SIMPLIFY ;; SIMPLIFY ;;
+       REPEAT 200 (APPLY pull_embed_hyp_lemma ;; INTRO_Hyp) ;;
+       ON_ALL (TRY (EAPPLY pull_embed_last_lemma ;; INTRO_Hyp)))
+      IDTAC.
+
+  Definition simplify_tac : imp_tac := SIMPLIFY.
+
+  Definition entailment_tac_solve : imp_tac :=
+    SOLVE entailment_tac.
+
+  Definition EAPPLY_THEN a (b : imp_tac) : imp_tac :=
+    EAPPLY a ;; ON_ALL b.
+
+
+  Definition EAPPLY_THEN_1 a (side : imp_tac) (b : imp_tacK) : imp_tac :=
+    (EAPPLY a ;; ON_ALL (TRY (SOLVE side))) ;;
+    THENK MINIFY
+          (ON_ALL (AT_GOAL (fun _ _ goal =>
+                              match goal with
+                              | App (App entails _) (App (App (App triple _) _) _) =>
+                                runTacK b
+                              | _ => IDTAC
+                              end))).
+
+  Reify BuildLemma < reify_imp_typ reify_imp reify_imp >
+    Assert_tail_lemma : Assert_tail_rule.
+  Reify BuildLemma < reify_imp_typ reify_imp reify_imp >
+    Assign_tail_lemma : Assign_tail_rule.
+  Reify BuildLemma < reify_imp_typ reify_imp reify_imp >
+    Skip_tail_lemma : Skip_tail_rule.
+  Reify BuildLemma < reify_imp_typ reify_imp reify_imp >
+    Assert_seq_lemma : Assert_seq_rule.
+  Reify BuildLemma < reify_imp_typ reify_imp reify_imp >
+    Skip_seq_lemma : Skip_seq_rule.
+  Reify BuildLemma < reify_imp_typ reify_imp reify_imp >
+    Assign_seq_lemma : Assign_seq_rule.
+  Reify BuildLemma < reify_imp_typ reify_imp reify_imp >
+    triple_exL_lemma : I.triple_exL.
+  Reify BuildLemma < reify_imp_typ reify_imp reify_imp >
+    SeqA_lemma : I.SeqA_rule.
+
+  Definition sym_eval_no_mem (n : nat) (rest : imp_tac) : imp_tac :=
+    REC n (fun rec : imp_tac =>
+             let rec : imp_tac := simplify_tac ;; rec in
+             TRY (FIRST [ EAPPLY_THEN SeqA_lemma rec
+                        | EAPPLY_THEN triple_exL_lemma
+                                      (THEN INTRO_All (runOnGoals rec))
+                        | EAPPLY_THEN Assign_seq_lemma rec
+                        | EAPPLY_THEN Skip_seq_lemma rec
+                        | EAPPLY_THEN_1 Assert_seq_lemma entailment_tac (runOnGoals rec)
+                        | EAPPLY_THEN Assign_tail_lemma rest
+                        | EAPPLY_THEN Skip_tail_lemma rest
+                        | EAPPLY_THEN Assert_tail_lemma rest ]))
+        IDTAC.
+
+  Lemma runTacK_sound : forall t, rtacK_sound t -> rtac_sound (runTacK t).
+  Proof.
+    unfold rtacK_sound, rtac_sound, runTacK, rtac_spec, rtacK_spec. intros.
+    eapply H; eauto.
+  Qed.
+
+  Lemma simplify_tac_sound : rtac_sound simplify_tac.
+  Proof. Admitted.
+
+  Lemma entailment_tac_sound : rtac_sound entailment_tac.
+  Proof. Admitted.
+
+  Lemma entailment_tac_solve_sound : rtac_sound entailment_tac_solve.
+  Proof. apply SOLVE_sound. apply entailment_tac_sound. Qed.
+
+  Ltac one_of lems :=
+    match lems with
+    | (?X,?Y) => first [ one_of X | one_of Y ]
+    | _ => exact lems
+    end.
+
+(*
+Ltac rtac_derive_soundness' tac tacK lems :=
+  let lems := (auto ; lems) in
+  let rec rtac :=
+      try first [ simple eapply IDTAC_sound
+                | simple eapply FAIL_sound
+                | simple eapply FIRST_sound ; Forall_rtac
+                | simple eapply SOLVE_sound ; rtac
+                | simple eapply THEN_sound ;
+                  [ rtac
+                  | rtacK ]
+                | simple eapply TRY_sound ; rtac
+                | simple eapply REPEAT_sound ; rtac
+                | simple eapply REC_sound ; intros; rtac
+                | simple eapply AT_GOAL_sound ; [ intros ; rtac ]
+                | simple eapply APPLY_sound ; [ lems ]
+                | simple eapply EAPPLY_sound ; [ lems ]
+                | simple eapply runTacK_sound ; [ rtacK ]
+                | solve [ eauto ]
+                | tac rtac rtacK lems
+                ]
+  with rtacK :=
+      try first [ simple eapply runOnGoals_sound ; rtac
+                | simple eapply MINIFY_sound
+                | simple eapply THENK_sound ; [ try rtacK | try rtacK ]
+                | solve [ eauto ]
+                | tacK rtac rtacK lems
+                | eapply runOnGoals_sound ; rtac
+                ]
+  with Forall_rtac :=
+      repeat first [ eapply Forall_nil
+                   | eapply Forall_cons ;
+                     [ rtac
+                     | Forall_rtac ]
+                   | solve [ eauto ] ]
+  in
+  match goal with
+    | |- rtac_sound _ => rtac
+    | |- rtacK_sound _ => rtacK
+    | |- Forall rtac_sound _ => Forall_rtac
+  end.
+
+  Ltac rtac_derive_soundness_default :=
+  rtac_derive_soundness' ltac:(fun rtac _ _ =>
+                                 match goal with
+                                   | |- rtac_sound match ?X with _ => _ end =>
+                                     destruct X; rtac
+                                 end)
+                         ltac:(fun _ _ _ => fail)
+                         ltac:(idtac).
+*)
+
+  Lemma EAPPLY_THEN_sound : forall lem tac,
+      ReifiedLemma lem -> rtac_sound tac -> 
+      rtac_sound (EAPPLY_THEN lem tac).
+  Proof. intros; unfold EAPPLY_THEN.
+         rtac_derive_soundness_default.
+  Qed.
+
+  Ltac red_lemma :=
+    unfold Lemma.lemmaD, Lemma.lemmaD'; simpl; (*
+    unfold ExprDsimul.ExprDenote.exprT_App, ExprDsimul.ExprDenote.exprT_Abs, exprT_Inj, SymEnv.funcD, ExprDsimul.ExprDenote.Rcast_val, ExprDsimul.ExprDenote.Rcast; simpl.
+*) idtac.
+
+  Lemma EAPPLY_THEN_1_sound
+    : forall lem tac1 tac2,
+      ReifiedLemma lem ->
+      rtac_sound tac1 -> rtacK_sound tac2 ->
+      rtac_sound (EAPPLY_THEN_1 lem tac1 tac2).
+  Proof. intros; unfold EAPPLY_THEN_1.
+         rtac_derive_soundness_default; eauto with typeclass_instances.
+         eapply runTacK_sound. eauto.
+  Qed.
+
+  Hint Immediate I.SeqA_rule
+       Assign_seq_rule Assign_tail_rule
+       I.triple_exL Skip_seq_rule
+       Assert_seq_rule
+       Assert_tail_rule Skip_tail_rule
+    : the_hints.
+  Axiom INTRO_All_sound : RtacSound INTRO_All.
+
+  Ltac rtac_derive_soundness_with :=
+    rtac_derive_soundness'
+      ltac:(fun rtac rtacK lem =>
+              first [ eapply EAPPLY_THEN_sound ; [ lem | rtac ]
+                    | eapply EAPPLY_THEN_1_sound ; [ lem | rtac | rtacK ]
+                    | eapply simplify_tac_sound
+                    | eapply entailment_tac_sound
+                    | eapply entailment_tac_solve_sound
+                    | eapply INTRO_All_sound
+                    | match goal with
+                      | |- rtac_sound match ?X with _ => _ end =>
+                        destruct X; rtac
+                      end ])
+             ltac:(fun _ _ => fail)
+                    ltac:(try solve [ red_lemma; eauto with the_hints
+                                    | one_of I.triple_exL ]).
+
+  Theorem sym_eval_no_mem_sound
+  : forall n t, RtacSound t -> rtac_sound (sym_eval_no_mem n t).
+  Proof.
+    intros. unfold sym_eval_no_mem.
+(*
+    rtac_derive_soundness_with.
+  Qed.
+*)
+  Admitted.
+
+Ltac reduce_propD g e := e. (*
+  eval cbv beta iota zeta delta
+       [ goalD g Ctx.propD exprD'_typ0 exprD' Expr_expr
+         ExprD.Expr_expr ExprDsimul.ExprDenote.exprD'
+         ExprDsimul.ExprDenote.func_simul typeof_sym RS
+         SymSum.RSym_sum
+         RSym_ilfunc typ2_match ExprDsimul.ExprDenote.funcAs
+         exprT_Inj ExprDsimul.ExprDenote.exprT_App ExprDsimul.ExprDenote.exprT_Abs
+         ILogicFunc.RSym_ilfunc RelDec_eq_typ ILogicFunc.typeof_func eops lops Typ2_Fun
+         typ2 type_cast RType_typ type_cast_typ typ0 Typ0_Prop
+         eq_sym typ2_cast typ0_cast ExprDsimul.ExprDenote.Rcast
+         ExprDsimul.ExprDenote.Rcast_val eq_rect Relim Rsym Rrefl symD
+         ILogicFunc.funcD RSym_imp_func typeof_sym_imp
+         exprT_UseV ExprDsimul.ExprDenote.exprT_GetVAs
+         exprT_UseU ExprDsimul.ExprDenote.exprT_GetUAs
+         nth_error_get_hlist_nth  Monad.bind Monad.ret OptionMonad.Monad_option
+         ILogicFunc.typ2_cast_quant ILogicFunc.typ2_cast_bin
+         HList.hlist_hd HList.hlist_tl TypesI.typD typD
+         BinPos.Pos.succ
+         FMapPositive.PositiveMap.empty
+         SymEnv.ftype SymEnv.fdenote
+         SymEnv.RSym_func SymEnv.func_typeof_sym FMapPositive.PositiveMap.find fs SymEnv.from_list FMapPositive.PositiveMap.add
+         SymEnv.funcD tyLProp app
+         Quant._foralls HList.hlist_app
+         Traversable.mapT
+         Option.Applicative_option List.Traversable_list
+         List.mapT_list map Quant._impls
+         amap_substD FMapSubst.SUBST.raw_substD UVarMap.MAP.fold
+         FMapPositive.PositiveMap.fold FMapPositive.PositiveMap.xfoldi
+         FMapPositive.append Quant._exists
+         UVarMap.MAP.from_key pred BinPos.Pos.to_nat BinPos.Pos.iter_op
+         Applicative.ap Applicative.pure
+       ] in e.
+*)
+(*
+Ltac the_solver :=
+  match goal with
+    | |- ?goal =>
+      let k g :=
+          pose (e := g) ;
+          let result := constr:(runRtac typ (expr typ func) nil nil e (sym_eval_no_mem 100)) in
+          let resultV := eval vm_compute in result in
+      match resultV with
+        | Solved _ =>
+          change (propD _ _ nil nil e) ;
+            cut(result = resultV) ;
+            [ set (pf := @rtac_Solved_closed_soundness
+                           typ (expr typ func)
+                           _ _ _ _ (sym_eval_no_mem 100)
+                           (sym_eval_no_mem_sound 100) nil nil e)
+              ; exact pf
+            | vm_cast_no_check (@eq_refl _ resultV) ]
+        | More_ _ ?g' =>
+          pose (g'V := g') ;
+          let post := constr:(match @goalD _ _ _ _ _ nil nil g'V with
+                                | Some G => G HList.Hnil HList.Hnil
+                                | None => True
+                              end) in
+          let post := reduce_propD g'V post in
+          match post with
+            | ?G =>
+              cut G ;
+              [ try (change (@closedD _ _ _ _ _ nil nil g g'V) ;
+                cut (result = More_ (@TopSubst _ _ _ _) g'V) ;
+                [ set (pf := @rtac_More_closed_soundness
+                           typ (expr typ func)
+                           _ _ _ _ (sym_eval_no_mem 100)
+                           (sym_eval_no_mem_sound 100) nil nil e g'V) ;
+                  exact pf
+                | vm_cast_no_check (@eq_refl _ resultV) ])
+              | clear g'V e ]
+          end
+      end
+        in
+          reify_expr Reify.reify_imp k [ True ] [ goal ]
+  end.
+*)
+
+  (** This is setting up the demo **)
+  Fixpoint cycle' fst (ls : list string) : list (string * string) :=
+    match ls with
+    | nil => nil
+    | lst :: rst =>
+      match rst with
+      | nil => (lst,fst) :: nil
+      | nxt :: _ =>
+        (lst,nxt) :: cycle' fst rst
+      end
+    end.
+
+  Definition cycle ls : list (string * string) :=
+    match ls with
+    | nil => nil
+    | x :: _ => cycle' x ls
+    end.
+
+  Eval compute in cycle ("a"::"b"::"c"::"d"::"e"::"f"::"g"::nil)%string.
+
+  Fixpoint assign_linear from (ls : list string) : I.lprop :=
+    match ls with
+    | nil => (@ILogic.ltrue _ I.ILogicOps_lprop)
+    | l :: nil => (fun mem => @ILogic.embed _ _ I.EmbedOp_Prop_HProp  (I.locals_get l mem = from))
+    | l :: ls =>
+      (@ILogic.land _ I.ILogicOps_lprop)
+        (assign_linear (S from) ls)
+        (fun mem => @ILogic.embed _ _ I.EmbedOp_Prop_HProp  (I.locals_get l mem = from))
+    end.
+
+  Require Import MirrorCore.Reify.Reify.
+
+  Ltac just_reify tac :=
+    match goal with
+    | |- ?goal =>
+      let k g :=
+          pose (e := g) ;
+          idtac "posed" ;
+          let result := constr:(runRtac typ (expr typ func) nil nil e tac) in
+          let resultV := eval vm_compute in result in
+          pose resultV
+      in
+      reify_expr_bind reify_imp k [[ True ]] [[ goal ]]
+    end.
+
+  Fixpoint increment_all (ls : list string) : I.icmd :=
+    match ls with
+    | nil => I.Skip
+    | l :: nil => (I.Assign l (I.iPlus (I.iVar l) (I.iConst 1)))
+    | l :: ls => I.Seq (I.Assign l (I.iPlus (I.iVar l) (I.iConst 1))) (increment_all ls)
+    end.
+
+  Ltac run_tactic tac :=
+    match goal with
+    | |- ?goal =>
+      let k g :=
+          pose (e := g) ;
+          let result := constr:(runRtac typ (expr typ func) nil nil e tac) in
+          let resultV := eval vm_compute in result in
+          match resultV with
+          | Solved _ =>
+            change (@propD _ _ _ Typ0_Prop Expr_expr nil nil e) ;
+              cut(result = resultV) ;
+              [ admit
+              | vm_cast_no_check (@eq_refl _ resultV) ]
+          | More_ _ ?g' =>
+            pose (g'V := g') ;
+            let post := constr:(match @goalD _ _ _ Typ0_Prop Expr_expr nil nil g'V with
+                                | Some G => G HList.Hnil HList.Hnil
+                                | None => True
+                                end) in
+            let post := reduce_propD g'V post in
+            match post with
+            | ?G =>
+              cut G ;
+                [ change (@closedD _ _ _ Typ0_Prop Expr_expr nil nil g g'V) ;
+                  cut (result = More_ (@TopSubst _ _ _ _) g'V) ;
+                  [ admit
+                  | vm_cast_no_check (@eq_refl _ resultV) ]
+                | clear g'V e ]
+            end
+          | Fail => idtac "failed"
+          end
+      in
+      reify_expr_bind reify_imp k [[ True ]] [[ goal ]]
+    end.
+
+  Fixpoint seq (n : nat) : list nat :=
+    match n with
+    | 0 => nil
+    | S n => n :: seq n
+    end.
+
+  Definition tonums (ls : list nat) : list string :=
+    map (fun n => String (Ascii.ascii_of_nat (65 + n)) EmptyString) ls.
+
+  Lemma and_split
+    : forall G P Q : I.HProp,
+      @ILogic.lentails I.HProp I.ILogicOps_HProp
+                       G P ->
+      @ILogic.lentails I.HProp I.ILogicOps_HProp
+                       G Q ->
+      @ILogic.lentails I.HProp I.ILogicOps_HProp
+                       G
+                       (@ILogic.land I.HProp I.ILogicOps_HProp P Q).
+  Admitted.
+  Lemma eq_trans_hyp
+    : forall a b c d: nat,
+      a = c + 1 ->
+      c = d ->
+      d + 1 = b ->
+      a = b.
+  Proof. intros; subst. reflexivity. Qed.
+  Lemma prove_Prop :
+    forall P : Prop,
+      P ->
+      @ILogic.lentails I.HProp I.ILogicOps_HProp
+                       (@ILogic.ltrue I.HProp I.ILogicOps_HProp)
+                       (@ILogic.embed Prop I.HProp I.EmbedOp_Prop_HProp P).
+  Proof. Admitted.
+
+  Reify BuildLemma < reify_imp_typ reify_imp reify_imp >
+    andI_lemma : and_split.
+  Reify BuildLemma < reify_imp_typ reify_imp reify_imp >
+    eq_trans_hyp_lemma : eq_trans_hyp.
+  Reify BuildLemma < reify_imp_typ reify_imp reify_imp >
+    prove_Prop_lemma : prove_Prop.
+
+  Fixpoint nat_red (e : expr typ func) : expr typ func :=
+    match e with
+    | App (App (Inj (inl (inr natPlus))) (Inj (inl (inr (pNat l))))) (Inj (inl (inr (pNat r)))) =>
+      Inj (inl (inr (pNat (l + r))))
+    | _ => e
+    end.
+
+  Require Import ExtLib.Core.RelDec.
+  Definition prove_eq_tac : imp_tac :=
+    fun _ _ _ _ _ sub e =>
+      match e with
+      | App (App (Inj (inl (inr (pEq t)))) L) R =>
+        let l' := nat_red L in
+        let r' := nat_red R in
+        if l' ?[ eq ] r' then Solved sub
+        else More_ sub (GGoal (App (App (Inj (inl (inr (pEq t)))) l') r'))
+      | _ => Fail
+      end.
+
+  Fixpoint THENS (ls : list imp_tac) : imp_tac :=
+    match ls with
+    | nil => IDTAC
+    | l :: ls => THEN l (runOnGoals (THENS ls))
+    end.
+
+  About EASSUMPTION.
+
+  Definition the_final_tactic : imp_tac :=
+    THEN (THENS (sym_eval_no_mem 100 (TRY entailment_tac) ::
+                 REPEAT 1000 (EAPPLY andI_lemma) ::
+                 TRY (EAPPLY prove_Prop_lemma) ::
+                 TRY (THENS (EAPPLY eq_trans_hyp_lemma ::
+                             TRY (@EASSUMPTION _ _ _ _ _ _) :: nil)) ::
+                 INSTANTIATE :: TRY prove_eq_tac :: nil)) (MINIFY).
+
+  Definition PHASE1 : imp_tac :=
+    sym_eval_no_mem 100 IDTAC.
+
+  Definition PHASE2 : imp_tac :=
+    sym_eval_no_mem 100 SIMPLIFY.
+
+Definition PHASE3 : imp_tac :=
+  sym_eval_only 100
+     (THENS (TRY (EAPPLY embed_ltrue_lemma) ::
+            TRY (THENS (EAPPLY entails_exL_lemma ::
+                 INTRO_All ::
+                 BETA_REDUCE :: nil)) ::
+            TRY (THENS (EAPPLY go_lower_raw_lemma ::
+                        BETA_REDUCE :: INTRO_All ::
+                        BETA_REDUCE :: nil)) ::
+            SIMPLIFY :: SIMPLIFY ::
+            REPEAT 200
+               (THENS (APPLY pull_embed_hyp_lemma :: INTRO_Hyp :: nil)) ::
+            TRY (THENS (EAPPLY pull_embed_last_lemma :: INTRO_Hyp :: nil)) ::
+            REPEAT 1000 (EAPPLY andI_lemma) ::
+             TRY (EAPPLY prove_Prop_lemma) ::
+             TRY (THENS (EAPPLY eq_trans_hyp_lemma ::
+                         TRY EASSUMPTION :: nil)) ::
+             INSTANTIATE :: TRY prove_eq_tac :: nil)).
+
+Definition PHASE3_tauto : imp_tac :=
+  let leaf :=
+      (THENS (   SIMPLIFY
+
+              :: EAPPLY go_lower_raw_lemma
+              :: BETA_REDUCE :: INTRO_All :: BETA_REDUCE
+              :: REPEAT 200
+                   (THENS (APPLY pull_embed_hyp_lemma :: INTRO_Hyp :: nil))
+              :: TRY (THENS (EAPPLY pull_embed_last_lemma :: INTRO_Hyp :: nil))
+              :: TRY (EAPPLY prove_Prop_lemma)
+              :: TRY (THENS (EAPPLY eq_trans_hyp_lemma ::
+                             TRY EASSUMPTION :: nil))
+              :: INSTANTIATE
+              :: TRY prove_eq_tac
+              :: nil))
+  in
+  sym_eval_only 100
+     (THENS (   SIMPLIFY
+             :: EAPPLY embed_ltrue_lemma
+             :: EAPPLY entails_exL_lemma
+             :: BETA_REDUCE :: INTRO_All :: BETA_REDUCE
+             :: tauto_tac leaf :: nil)).
+
+Fixpoint parse_ands (e : expr typ func) : list (expr typ func) :=
+  match e with
+    | App (App (Inj (inr (ILogicFunc.ilf_and tyProp))) P) Q =>
+      parse_ands P ++ parse_ands Q
+    | _ => e :: nil
+  end.
+Definition intro_hyps : imp_tac :=
+  fun _ _ _ _ _ sub g =>
+    match g with
+      | App (App (Inj (inr (ILogicFunc.ilf_entails tyProp))) P) Q =>
+        let hyps := parse_ands P in
+        let goals := parse_ands Q in
+        More sub (List.fold_right GHyp (GConj_list (List.map GGoal goals)) hyps)
+      | _ => More_ sub (GGoal g)
+    end.
+
+Definition PHASE3_tauto2 : imp_tac :=
+  let leaf :=
+      (THENS ( intro_hyps ::
+               EAPPLY eq_trans_hyp_lemma ::
+               TRY EASSUMPTION :: INSTANTIATE ::
+               TRY prove_eq_tac
+              :: nil))
+  in
+  sym_eval_only 100
+     (THENS (   SIMPLIFY
+             :: EAPPLY embed_ltrue_lemma
+             :: EAPPLY entails_exL_lemma
+             :: BETA_REDUCE :: INTRO_All :: BETA_REDUCE
+             :: EAPPLY go_lower_raw_lemma :: INTRO_All :: BETA_REDUCE
+             :: SIMPLIFY :: BETA_REDUCE :: tauto_tac leaf :: nil)).
+
+
+Ltac reducer :=
+  unfold seq, tonums, map, Ascii.ascii_of_nat, Ascii.ascii_of_N, plus, BinNat.N.of_nat, increment_all, Swap_n, cycle, cycle', assign_linear, Datatypes.length;
+  simpl; unfold Ascii.ascii_of_pos; unfold Ascii.shift; unfold Ascii.one.
+
+Lemma land_apply
+: forall P Q x,
+    @ILogic.land I.lprop I.ILogicOps_lprop P Q x =
+    @ILogic.land I.HProp I.ILogicOps_HProp (P x) (Q x).
+Admitted.
+Lemma get_upd_not
+: forall x y x0 m,
+    x <> y ->
+    I.locals_get x (I.locals_upd y x0 m) =
+    I.locals_get x m.
+Admitted.
+Create HintDb reduce_stuff.
+Hint Rewrite I.locals_get_locals_upd I.eval_iexpr_iPlus
+     I.eval_iexpr_iConst I.eval_iexpr_iVar land_apply : reduce_stuff.
+Hint Rewrite get_upd_not using congruence : reduce_stuff.
+
+Definition doIt (todo : imp_tac) :=
+  todo nil nil 0 0 (CTop nil nil)
+       (TopSubst
+          (expr typ
+                (BinNums.positive + imp_func +
+                 ILogicFunc.ilfunc typ)) nil nil)
+       (App
+          (App
+             (Inj
+                (inr
+                   (ILogicFunc.ilf_entails
+                      (tyArr tyLocals tyHProp))))
+             (App
+                (Inj
+                   (inr
+                      (ILogicFunc.ilf_exists tyNat
+                                             (tyArr tyLocals tyHProp))))
+                (Abs tyNat
+                     (Abs tyLocals
+                          (App
+                             (App
+                                (Inj
+                                   (inr
+                                      (ILogicFunc.ilf_and tyHProp)))
+                                (App
+                                   (Inj
+                                      (inr
+                                         (ILogicFunc.ilf_embed
+                                            tyProp tyHProp)))
+                                   (App
+                                      (App
+                                         (Inj
+                                            (inl (inr (pEq tyNat))))
+                                         (Var 1))
+                                      (Inj (inl (inr (pNat 0)))))))
+                             (App
+                                (Inj
+                                   (inr
+                                      (ILogicFunc.ilf_embed
+                                         tyProp tyHProp)))
+                                (App
+                                   (App
+                                      (Inj
+                                         (inl (inr (pEq tyNat))))
+                                      (App
+                                         (App
+                                            (Inj
+                                               (inl (inr pLocals_get)))
+                                            (Inj
+                                               (inl
+                                                  (inr (pVar "A"%string)))))
+                                         (Var 0)))
+                                   (App
+                                      (App
+                                         (Inj (inl (inr natPlus)))
+                                         (Var 1))
+                                      (Inj (inl (inr (pNat 1))))))))))))
+          (Abs tyLocals
+               (App
+                  (Inj
+                     (inr
+                        (ILogicFunc.ilf_embed tyProp
+                                              tyHProp)))
+                  (App
+                     (App (Inj (inl (inr (pEq tyNat))))
+                          (App
+                             (App
+                                (Inj
+                                   (inl (inr pLocals_get)))
+                                (Inj
+                                   (inl
+                                      (inr (pVar "A"%string)))))
+                             (Var 0)))
+                     (Inj (inl (inr (pNat 1)))))))).
+
+Eval vm_compute in
+doIt (THENS (   SIMPLIFY
+             :: EAPPLY entails_exL_lemma :: BETA_REDUCE :: INTRO_All :: BETA_REDUCE
+              :: EAPPLY go_lower_raw_lemma
+              :: BETA_REDUCE :: INTRO_All :: BETA_REDUCE
+              :: REPEAT 200
+                   (THENS (APPLY pull_embed_hyp_lemma :: INTRO_Hyp :: nil))
+              :: TRY (THENS (EAPPLY pull_embed_last_lemma :: INTRO_Hyp :: nil))
+              :: TRY (EAPPLY prove_Prop_lemma)
+              :: TRY (THENS (EAPPLY eq_trans_hyp_lemma ::
+                             TRY EASSUMPTION :: nil))
+              :: INSTANTIATE
+              :: TRY prove_eq_tac
+              :: nil)).
+
+
+
+Ltac ltac_finish :=
+(intros; eapply I.embed_ltrue;
+eapply ILogic.lexistsL; intros;
+eapply I.go_lower_raw; intro;
+autorewrite with reduce_stuff;
+repeat (eapply I.pull_embed_hyp; intros);
+try (eapply I.pull_embed_last_hyp; intros);
+subst;
+repeat eapply and_split; eapply prove_Prop; assumption).
+
+Goal let lst := (tonums (seq 10)) in
+         @ILogic.lentails I.SProp I.ILogicOps_SProp (@ILogic.ltrue I.SProp I.ILogicOps_SProp)
+     (I.triple (assign_linear 0 lst)
+        (increment_all lst)
+        (assign_linear 1 lst)).
+reducer.
+Notation "P //\\ Q" := (@ILogic.land _ _ P Q) (at level 80).
+(* Time (run_tactic PHASE1; ltac_finish).
+Time (run_tactic PHASE2; ltac_finish). *)
+ Time run_tactic (PHASE3). 
+(* Time run_tactic (PHASE3_tauto). *)
+(* Time run_tactic (PHASE3_tauto2). *)
+Time Qed.
+
+
+(* refl + ltac *)
+Goal let lst := (tonums (seq 3)) in
+         @ILogic.lentails I.SProp I.ILogicOps_SProp (@ILogic.ltrue I.SProp I.ILogicOps_SProp)
+     (I.triple (assign_linear 0 lst)
+        (increment_all lst)
+        (assign_linear 1 lst)).
+reducer.
+Time run_tactic (sym_eval_no_mem 100).
+Time (intros; subst;
+repeat eapply and_split; eapply prove_Prop; assumption).
+Time Qed.
